compiler/dsl/coq/ReflexEcho.v
@@ -7,33 +7,35 @@ Require Import ReflexVec.
 
 Definition NB_MSG : nat := 1.
 
-Definition PAY_DESC : vvdesc NB_MSG :=
+Definition PAYD : vvdesc NB_MSG :=
   ( existT _ 1 (str_d, tt)
   , tt
   ).
 
-Definition INIT_ENVD : vdesc := existT _ 0 tt.
+Definition KSTD : vdesc := existT _ 0 tt.
 
-Definition INIT : @init_prog NB_MSG PAY_DESC INIT_ENVD :=
+Definition IENVD : vdesc := existT _ 0 tt.
+
+Definition INIT : init_prog PAYD KSTD IENVD :=
   nil.
 
-Definition KST_DESC : vdesc := existT _ 0 tt.
-
-Definition HANDLERS : handlers (VVD := PAY_DESC) (projT2 KST_DESC) :=
+Definition HANDLERS : handlers PAYD KSTD :=
   (fun m =>
-    match tag m as _tm return
-      @sdenote _ SDenoted_vdesc (lkup_tag (VVD := PAY_DESC) _tm) -> _
+    match tag PAYD m as _tm return
+      @sdenote _ SDenoted_vdesc (lkup_tag PAYD _tm) -> _
     with
     | None => fun pl =>
        let envd := existT _ 0 tt in
-       existT (fun d => hdlr_prog (projT2 KST_DESC) d) envd (fun cm cfd s =>
+       existT (fun d => hdlr_prog PAYD KSTD d) envd (fun cfd s =>
         let (s, _) := pl in
-        Send (VVD := PAY_DESC) envd (CFd _) None (SLit _ s, tt)
-        :: nil
+        (fun st0 =>
+           (fun st => Send PAYD envd (CFd _) None (SLit _ s, tt))
+           :: nil
+        )
       )
     | Some bad => fun _ =>
       match bad with end
-    end (pay m)
+    end (pay PAYD m)
   ).
 
-Definition main := mk_main (Build_spec NB_MSG PAY_DESC INIT_ENVD INIT KST_DESC HANDLERS).
+Definition main := mk_main (Build_spec NB_MSG PAYD IENVD KSTD INIT HANDLERS).
